\documentclass[11pt]{article}
\usepackage{fullpage,amsmath}

% --- -----------------------------------------------------------------
% --- Document-specific definitions.
% --- -----------------------------------------------------------------
\newtheorem{definition}{Definition}

\newcommand{\concat}{{\,\|\,}}
\newcommand{\bits}{\{0,1\}}

% --- -----------------------------------------------------------------
% --- The document starts here.
% --- -----------------------------------------------------------------
\begin{document}
\sloppy

\noindent Rutgers University\\
CS440: Introduction to Artificial Intelligence, Spring 2017\\
Kostas Bekris\\

\begin{center}
\LARGE{\textbf{Homework 3: James Carroll and Joel Carrillo}}\\
\large{\textbf{\emph{Bayesian Inference, Temporal State Estimation and Decision Making under Uncertainty}}}
\end{center}

\vspace{.1in}

\begin{enumerate}

\item Question 1
\begin{enumerate}

\item a) 
\begin{enumerate}
\item $P(A, B, C, D, E) =$
\item $P(A)P(B)P(C)P(D|A,B)P(E|B,C) =$
\item $(0.2)(0.5)(0.8)(0.1)(0.3) = 0.0024$
\end{enumerate}

\item b) 
\begin{enumerate}
\item $P(\neg A)P(\neg B)P(\neg C)P(\neg D)P(\neg E) =$ 
\item $P(\neg A)P(\neg B)P(\neg C)P(\neg D|\neg A, \neg B)P(\neg E|\neg B, \neg C) =$
\item $(1 - 0.2)(1 - 0.5)(1 - 0.8)(1 - 0.9)(1 - 0.2) =$ 
\item $(0.8)(0.5)(0.2)(0.1)(0.8) = 0.0064$
\end{enumerate}

\item c) 
\begin{enumerate}
\item $P(\neg A | B, C, D, E) =\frac{P(\neg A, B, C, D, E)}{P(\neg A, B, C, D, E) + P(A, B, C, D, E)}$ 
\item  $P(\neg A, B, C, D, E) = P(\neg A)P(B)P(C)P(D |\neg A, B)P(E | B, C) = $ \item $(0.8)(0.5)(0.8)(0.6)(0.3) = 0.0576$ 
\item $\frac{0.0576}{0.0576+0.0024} = 0.96$
\end{enumerate}

\end{enumerate}

\item Question 2
\begin{enumerate}
\item $P(Burglary|JohnCalls = true, MaryCalls = true)$
\\Factors:$ P(Burglary), P(EQ)$, $P(Alarm|EQ, Burglary)$,$ P(JohnCalls|Alarm)$, $P(MaryCalls|Alarm)$
\\Elimination Order: EQ, Alarm
\\
\\$f_{1}(Alarm, Burglary) = \sum_{EQ} P(EQ) P(Alarm, EQ, Burglary)$
\\$f_{2}(John, Mary, Alarm, EQ) = \sum_{Alarm}f_{1}(Alarm,Burglary)P(John|Alarm)P(Mary|Alarm)$
\\$P(Burglary|JohnCalls,MaryCalls) = P(Burglary)f_{2}(John, Mary, Alarm, Burglary)$
\\
\\Normalize the above to find $P(Burglary|JohnCalls = true, MaryCalls = true)$
\item
\item
\end {enumerate}

\item Question 3
\begin{enumerate}
\item a) 
\begin{enumerate}
\item By definition: $P(X|MB(X)) = P(X|Parents,Children,PofC) $
\item FJPD for parents: $P(Y_i, ..., Y_n) = \prod{i = 1}^{n} P(Y_i | Z_{i}1)$ 
\item All together: 
\end{enumerate}
\item b)
\item c)
\end{enumerate}

\item Question 4
\begin {enumerate}
\item
\item
\item
\item
\end {enumerate}

\item Question 5a

\item Question 5b

\item Question 5c

\item Question 5d

\item Question 5e

\item Question 5f

\item Question 5h

\end{enumerate}
\end{document}
